trying out some more transformations in swap

examples/dm4free/swap.fst
@@ -107,6 +107,37 @@ let idem (#rs #ws:addr_set) (f:cmd rs ws)
       () in                         
     FStar.Classical.forall_intro aux
 
+type guard' = unit -> STNull bool
+
+let guard_is_readonly (c:guard') =
+  forall (h:heap).
+    let _, h1 = reify ((c <: guard') ()) h in
+    h == h1
+
+type guard = g:guard'{guard_is_readonly g}
+
+reifiable let cond (c:guard) (c1:command) (c2:command) (_:unit) :STNull unit
+  = let b = (c <: guard) () in
+    if b then (c1 <: command) () else (c2 <: command) ()
+
+let lemma_replace_cond (c:guard) (c1:command) (c2:command)
+  :Lemma (requires (guard_is_readonly c /\ equiv c1 c2))
+         (ensures  (equiv (cond c c1 c2) c1 /\
+	            equiv (cond c c1 c2) c2))
+  = let aux (h:heap) :Lemma (equiv_on_h (cond c c1 c2) c1 h /\ equiv_on_h (cond c c1 c2) c2 h)
+      = let (), _ = reify ((c1 <: command) ()) h in
+        let (), _ = reify ((c2 <: command) ()) h in
+        ()
+    in
+    FStar.Classical.forall_intro aux
+
+let lemma_skip_c1 (#r1 #w1 #r2 #w2:addr_set) (c1:cmd r1 w1) (c2:cmd r2 w2) (h:heap)
+  :Lemma (requires (S.disjoint__ w1 r2 /\ S.subset w1 w2))
+         (ensures  (equiv_on_h (c1 >> c2) c2 h))
+  = let (), h1 = reify ((c1 <: command) ()) h in
+    let (), h2 = reify ((c2 <: command) ()) h in
+    ()
+
 (*** OLD ***)
 
 
